WebAssembly/Wasm_Interpreter_Properties.thy
@@ -1114,6 +1114,203 @@ next
     by fastforce
 qed
 
+lemma run_one_step_return_call:
+  assumes "run_one_step d i (s,vs,ves,e) = (s', vs', RSReturnCall c res)"
+  shows "(\<exists>j. e = $ReturnCall j) \<or> (\<exists>n les es. e = Label n les es)"
+proof (cases e)
+  case (Basic x1)
+  thus ?thesis
+  proof (cases x1)
+    case Unreachable
+    thus ?thesis
+      using run_one_step_basic_unreachable_result assms Basic
+      by fastforce
+  next
+    case Nop
+    thus ?thesis
+      using assms Basic
+      by fastforce
+  next
+    case Drop
+    thus ?thesis
+      using run_one_step_basic_drop_result assms Basic
+      by fastforce
+  next
+    case Select
+    thus ?thesis
+      using run_one_step_basic_select_result assms Basic
+      by fastforce
+  next
+    case (Block x51 x52)
+    thus ?thesis
+      using run_one_step_basic_block_result assms Basic
+      by fastforce
+  next
+    case (Loop x61 x62)
+    thus ?thesis
+      using run_one_step_basic_loop_result assms Basic
+      by fastforce
+  next
+    case (If x71 x72 x73)
+    thus ?thesis
+      using run_one_step_basic_if_result assms Basic
+      by fastforce
+  next
+    case (Br x8)
+    thus ?thesis
+      using run_one_step_basic_br_result assms Basic
+      by fastforce
+  next
+    case (Br_if x9)
+    thus ?thesis
+      using run_one_step_basic_br_if_result assms Basic
+      by fastforce
+  next
+    case (Br_table x10)
+    thus ?thesis
+      using run_one_step_basic_br_table_result assms Basic
+      by fastforce
+  next
+    case Return
+    thus ?thesis
+      using run_one_step_basic_return_result assms Basic
+      by fastforce
+  next
+    case (Call x12)
+    thus ?thesis
+      using run_one_step_basic_call_result assms Basic
+      by fastforce
+  next
+    case (Call_indirect x13)
+    thus ?thesis
+      using run_one_step_basic_call_indirect_result assms Basic
+      by fastforce
+  next
+    case (ReturnCall x12)
+    thus ?thesis
+      using run_one_step_basic_return_call_result assms Basic
+      by fastforce
+  next
+    case (ReturnCall_indirect x13)
+    thus ?thesis
+      using run_one_step_basic_return_call_indirect_result assms Basic
+      by fastforce
+  next
+    case (Get_local x14)
+    thus ?thesis
+      using run_one_step_basic_get_local_result assms Basic
+      by fastforce
+  next
+    case (Set_local x15)
+    thus ?thesis
+      using run_one_step_basic_set_local_result assms Basic
+      by fastforce
+  next
+    case (Tee_local x16)
+    thus ?thesis
+      using run_one_step_basic_tee_local_result assms Basic
+      by fastforce
+  next
+    case (Get_global x17)
+    thus ?thesis
+      using assms Basic
+      by fastforce
+  next
+    case (Set_global x18)
+    thus ?thesis
+      using run_one_step_basic_set_global_result assms Basic
+      by fastforce
+  next
+    case (Load x191 x192 x193 x194)
+    thus ?thesis
+      using run_one_step_basic_load_result assms Basic
+      by fastforce
+  next
+    case (Store x201 x202 x203 x204)
+    thus ?thesis
+      using run_one_step_basic_store_result assms Basic
+      by fastforce
+  next
+    case Current_memory
+    thus ?thesis
+      using run_one_step_basic_current_memory_result assms Basic
+      by fastforce
+  next
+    case Grow_memory
+    thus ?thesis
+      using run_one_step_basic_grow_memory_result assms Basic
+      by fastforce
+  next
+    case (EConst x23)
+    thus ?thesis
+      using assms Basic
+      by fastforce
+  next
+    case (Unop_i x241 x242)
+    thus ?thesis
+      using run_one_step_basic_unop_i_result assms Basic
+      by fastforce
+  next
+    case (Unop_f x251 x252)
+    thus ?thesis
+      using run_one_step_basic_unop_f_result assms Basic
+      by fastforce
+  next
+    case (ExtendS x241 x242)
+    thus ?thesis
+      using run_one_step_basic_extend_s_result assms Basic
+      by fastforce
+  next
+    case (Binop_i x261 x262)
+    thus ?thesis
+      using run_one_step_basic_binop_i_result assms Basic
+      by fastforce
+  next
+    case (Binop_f x271 x272)
+    thus ?thesis
+      using run_one_step_basic_binop_f_result assms Basic
+      by fastforce
+  next
+    case (Testop x281 x282)
+    thus ?thesis
+      using run_one_step_basic_testop_result assms Basic
+      by fastforce
+  next
+    case (Relop_i x291 x292)
+    thus ?thesis
+      using run_one_step_basic_relop_i_result assms Basic
+      by fastforce
+  next
+    case (Relop_f x301 x302)
+    thus ?thesis
+      using run_one_step_basic_relop_f_result assms Basic
+      by fastforce
+  next
+    case (Cvtop x311 x312 x313 x314)
+    thus ?thesis
+      using run_one_step_basic_cvtop_result assms Basic
+      by fastforce
+  qed
+next
+  case Trap
+  thus ?thesis
+    using assms
+    by auto
+next
+  case (Callcl x3)
+  thus ?thesis
+    using assms run_one_step_callcl_result
+    by fastforce
+next
+  case (Label x41 x42 x43)
+  thus ?thesis
+    by auto
+next
+  case (Local x51 x52 x53 x54)
+  thus ?thesis
+    using assms run_one_step_local_result
+    by fastforce
+qed
 lemma run_one_step_return:
   assumes "run_one_step d i (s,vs,ves,e) = (s', vs', RSReturn res)"
   shows "(e = $Return) \<or> (\<exists>n les es. e = Label n les es)"
@@ -1362,6 +1559,31 @@ proof -
     by blast
 qed
 
+lemma run_step_return_call_imp_not_trap_const_list:
+  assumes "run_step d i (s, vs, es) = (s', vs', RSReturnCall c res)"
+  shows "es \<noteq> [Trap]" "\<not>const_list es"
+proof -
+  {
+    assume "es = [Trap]"
+    hence False
+      using assms
+      by simp
+  }
+  thus "es \<noteq> [Trap]"
+    by blast
+  {
+    assume "const_list es"
+    then obtain vs where "split_vals_e es = (vs, [])"
+      using split_vals_e_const_list e_type_const_conv_vs
+      by fastforce
+    hence False
+      using assms
+      by simp
+  }
+  thus "\<not>const_list es"
+    by blast
+qed
+
 lemma run_one_step_label_break_imp_break:
   assumes "run_one_step d i (s, vs, ves, Label ln les es) = (s', vs', RSBreak n res)"
   shows "run_step d i (s, vs, es) = (s', vs', RSBreak (Suc n) res)"
@@ -1383,6 +1605,25 @@ qed auto
 lemma run_one_step_label_return_imp_return:
   assumes "run_one_step d i (s, vs, ves, Label n les es) = (s', vs', RSReturn res)"
   shows "run_step d i (s, vs, es) = (s', vs', RSReturn res)"
+  using assms
+proof (cases "es = [Trap]"; cases "const_list es")
+  assume local_assms:"es \<noteq> [Trap]" "\<not>const_list es"
+  obtain s'' vs'' res'' where rs_def:"run_step d i (s, vs, es) = (s'', vs'', res'')"
+    by (metis surj_pair)
+  thus ?thesis
+    using assms local_assms
+  proof (cases res'')
+    case (RSBreak x21 x22)
+    thus ?thesis
+      using assms local_assms rs_def
+      by (cases x21; cases "n \<le> length x22") auto
+  qed auto
+qed auto
+thm run_step_run_one_step.induct
+
+lemma run_one_step_label_return_call_imp_return:
+  assumes "run_one_step d i (s, vs, ves, Label n les es) = (s', vs', RSReturnCall c res)"
+  shows "run_step d i (s, vs, es) = (s', vs', RSReturnCall c res)"
   using assms
 proof (cases "es = [Trap]"; cases "const_list es")
   assume local_assms:"es \<noteq> [Trap]" "\<not>const_list es"
@@ -1589,6 +1830,87 @@ proof -
         by fastforce
       thus ?thesis
         using 2(3) 2(1)[OF e_def _ run_step_return_imp_not_trap_const_list(2)] e_def
+        by fastforce
+    qed
+  qed
+  thus ?thesis
+    using assms
+    by blast
+qed
+
+lemma run_step_return_call_imp_lfilled:
+  assumes "run_step d i (s,vs,es) = (s', vs', RSReturnCall c res)"
+  shows "s = s' \<and> vs = vs' \<and> (\<exists>n lfilled es_c. Lfilled_exact n lfilled ((vs_to_es res) @ [$Return] @ es_c) es)"
+proof -
+  fix ves e
+  have "(run_step d i (s,vs,es) = (s', vs', RSReturnCall c res)) \<Longrightarrow>
+           s = s' \<and> vs = vs' \<and> (\<exists>n lfilled j es_c. Lfilled_exact n lfilled ((vs_to_es res) @ [$ReturnCall j] @ es_c) es)"
+  and  "(run_one_step d i (s,vs,ves,e) = (s', vs', RSReturnCall c res)) \<Longrightarrow>
+          s = s' \<and> vs = vs' \<and>
+          (\<exists>j. (res = ves \<and> e = ($ReturnCall j)) \<or>
+           (\<exists>n lfilled j ves es_c es n' les'. Lfilled_exact n lfilled ((vs_to_es res) @ [$ReturnCall j] @ es_c) es \<and>
+              e = Label n' les' es))"
+  proof (induction d i "(s,vs,es)" and d i "(s,vs,ves,e)" arbitrary: s vs es s' vs' res and s vs ves e s' vs' res rule: run_step_run_one_step.induct)
+    case (1 d i s vs es)
+    obtain ves es' where split_vals_es:"split_vals_e es = (ves, es')"
+      by (metis surj_pair)
+    then obtain a as where es'_def:"es' = a#as"
+      using 1(2)
+      by (cases es') auto
+    hence a_def:"\<not> e_is_trap a"
+      using 1(2) split_vals_es
+      by (cases "a = Trap"; cases "(as \<noteq> [] \<or> ves \<noteq> [])") simp_all
+    obtain s'' vs'' res'' where "run_one_step d i (s,vs,(rev ves),a) = (s'', vs'', res'')"
+      by (metis surj_pair)
+    hence ros_def:"run_one_step d i (s,vs,(rev ves),a) = (s', vs', RSReturnCall c res)"
+      using 1(2) split_vals_es es'_def a_def
+      by (cases "res''") (auto simp del: run_one_step.simps)
+    obtain n lfilled j les_c les n' les' where
+      "s = s'" "vs = vs'"
+      "(res = rev ves \<and> a = $ReturnCall j) \<or> (Lfilled_exact n lfilled ((vs_to_es res) @ [$ReturnCall j] @ les_c) les \<and> a = Label n' les' les)"
+      using 1(1)[OF split_vals_es[symmetric] _ es'_def a_def ros_def]
+      by fastforce
+    then consider
+      (1) "s = s'" "vs = vs'" "res = rev ves" "a = $ReturnCall j"
+    | (2) "s = s'" "vs = vs'" "(Lfilled_exact n lfilled ((vs_to_es res) @ [$ReturnCall j] @ les_c) les)" "(a = Label n' les' les)"
+      by blast
+    thus ?case
+    proof cases
+      case 1
+      thus ?thesis
+        using es'_def split_vals_e_conv_app[OF split_vals_es] Lfilled_exact.intros(1) is_const_list[of _ ves]
+        by fastforce
+    next
+      case 2
+      have "const_list ($$* ves)"
+        using is_const_list
+        by fastforce
+      thus ?thesis
+        using 2 Lfilled_exact.intros(2) es'_def split_vals_e_conv_app[OF split_vals_es]
+          by fastforce
+    qed
+  next
+    case (2 d i s vs ves e s' vs')
+    consider (a) "(\<exists>j. e = $ReturnCall j)" | (b) "(\<exists>n les es. e = Label n les es)"
+      using run_one_step_return_call[OF 2(3)]
+      by blast
+    thus ?case
+    proof cases
+      case a
+      thus ?thesis
+        using 2(3)
+        by simp
+    next
+      case b
+      then obtain n les es where e_def:"e = Label n les es"
+        by blast
+      hence "run_one_step d i (s, vs, ves,  Label n les es) = (s', vs', RSReturnCall c res)"
+        using 2(3) by simp
+      hence "run_step d i (s, vs, es) = (s', vs', RSReturnCall c res)"
+        using run_one_step_label_return_call_imp_return
+        by fastforce
+      thus ?thesis
+        using 2(3) 2(1)[OF e_def _ run_step_return_call_imp_not_trap_const_list(2)] e_def
         by fastforce
     qed
   qed
@@ -2011,7 +2333,7 @@ proof -
         by fastforce
       thus ?thesis
         using assms Get_local True
-              progress_L0_left[OF reduce.intros(8)]
+              progress_L0_left[OF reduce.intros(11)]
               is_const_list_vs_to_es_list[of "rev ves"]
         by auto
     qed auto
@@ -2030,7 +2352,7 @@ proof -
           by fastforce
         thus ?thesis
           using assms Set_local True Cons
-                progress_L0_left[OF reduce.intros(9)]
+                progress_L0_left[OF reduce.intros(12)]
                 is_const_list_vs_to_es_list[of "rev list"]
           by auto
       qed auto
@@ -2051,7 +2373,7 @@ proof -
     case (Get_global x17)
     thus ?thesis
       using assms
-            progress_L0_left[OF reduce.intros(10)]
+            progress_L0_left[OF reduce.intros(13)]
             is_const_list_vs_to_es_list[of "rev ves"]
       by (auto simp add: is_const_def)
   next
@@ -2062,7 +2384,7 @@ proof -
       case (Cons a list)
       thus ?thesis
         using assms Set_global
-              progress_L0_left[OF reduce.intros(11)]
+              progress_L0_left[OF reduce.intros(14)]
               is_const_list_vs_to_es_list[of "rev list"]
         by (auto simp add: is_const_def)
     qed auto
@@ -2080,8 +2402,8 @@ proof -
         case (Some a)
         thus ?thesis
           using Load assms None Cons ConstInt32
-              progress_L0_left[OF reduce.intros(12)]
-              progress_L0_left[OF reduce.intros(13)]
+              progress_L0_left[OF reduce.intros(15)]
+              progress_L0_left[OF reduce.intros(16)]
               is_const_list_vs_to_es_list[of "rev list"]
           by (cases "load (s.mem s ! a) (nat_of_int x1) x194 (t_length x191)" )
              (auto simp add: is_const_def)
@@ -2097,8 +2419,8 @@ proof -
           case (Some a)
           thus ?thesis
             using Load assms outer_some Cons ConstInt32 Pair
-                  progress_L0_left[OF reduce.intros(14)]
-                  progress_L0_left[OF reduce.intros(15)]
+                  progress_L0_left[OF reduce.intros(17)]
+                  progress_L0_left[OF reduce.intros(18)]
                   is_const_list_vs_to_es_list[of "rev list"]
             by (cases "load_packed sx (s.mem s ! a) (nat_of_int x1) x194 (tp_length tp) (t_length x191)")
                (auto simp add: is_const_def)
@@ -2128,8 +2450,8 @@ proof -
               case None
               thus ?thesis
                 using Store outer_Cons Cons assms True outer_Some ConstInt32
-                      progress_L0_left[OF reduce.intros(16)]
-                      progress_L0_left[OF reduce.intros(17)]
+                      progress_L0_left[OF reduce.intros(19)]
+                      progress_L0_left[OF reduce.intros(20)]
                       is_const_list_vs_to_es_list[of "rev list'"]
                 by (cases "store (s.mem s ! j) (nat_of_int x1) off (bits a) (t_length t)")
                    auto
@@ -2137,8 +2459,8 @@ proof -
               case (Some the_tp)
               thus ?thesis
                 using Store outer_Cons Cons assms True outer_Some ConstInt32
-                      progress_L0_left[OF reduce.intros(18)]
-                      progress_L0_left[OF reduce.intros(19)]
+                      progress_L0_left[OF reduce.intros(21)]
+                      progress_L0_left[OF reduce.intros(22)]
                       is_const_list_vs_to_es_list[of "rev list'"]
                 by (cases "store_packed (s.mem s ! j) (nat_of_int x1) off (bits a) (tp_length the_tp)")
                    auto
@@ -2155,7 +2477,7 @@ proof -
       case (Some a)
       thus ?thesis
         using assms Current_memory 
-              progress_L0_left[OF reduce.intros(20)]
+              progress_L0_left[OF reduce.intros(23)]
               is_const_list_vs_to_es_list[of "rev ves"]
         by (auto simp add: is_const_def)
     qed auto
@@ -2172,8 +2494,8 @@ proof -
         case (Some j)
         thus ?thesis
           using assms Grow_memory Cons ConstInt32
-                             progress_L0_left[OF reduce.intros(21)]
-                             progress_L0_left[OF reduce.intros(22)]
+                             progress_L0_left[OF reduce.intros(24)]
+                             progress_L0_left[OF reduce.intros(25)]
               is_const_list_vs_to_es_list[of "rev list"] 
           by (cases "mem_grow_impl (s.mem s ! j) (nat_of_int x1)") (auto simp add: mem_grow_impl_correct is_const_def)
       qed auto
@@ -2365,7 +2687,7 @@ proof -
             by auto
           moreover
           have "\<lparr>s;vs;(vs_to_es ves')@[Callcl cl]\<rparr> \<leadsto>_i \<lparr>s;vs;([Local (length t2s) i' (rev ves' @ (n_zeros fts)) [$Block ([] _> t2s) fes]])\<rparr>"
-            using reduce.intros(5) local_defs(1,2) Func_native ves'_length
+            using reduce.intros(8) local_defs(1,2) Func_native ves'_length
             unfolding cl_type_def
             by fastforce
           ultimately
@@ -2386,7 +2708,7 @@ proof -
               by auto
             thus ?thesis
               using is_const_list[of _ "(rev ves'')"]
-                    reduce.intros(7)[OF _ _ ves'_length local_defs(2)]
+                    reduce.intros(10)[OF _ _ ves'_length local_defs(2)]
                     split_n_conv_app[OF true_defs]
                     progress_L0_left Callcl Func_host local_defs(1)
               unfolding cl_type_def
@@ -2408,7 +2730,7 @@ proof -
                   unfolding cl_type_def
                   by auto
                 thus ?thesis
-                  using progress_L0_left reduce.intros(6)[OF _ _ ves'_length local_defs(2)] Pair
+                  using progress_L0_left reduce.intros(9)[OF _ _ ves'_length local_defs(2)] Pair
                         Callcl Func_host local_defs(1) True is_const_list[of _ "(rev ves'')"]
                         split_n_conv_app[OF true_defs] host_apply_impl_correct[OF Some]
                   unfolding cl_type_def
@@ -2617,23 +2939,20 @@ proof -
                 by auto
             next
               case (RSReturnCall x31 x32)
-              thus ?thesis
-              sorry
-            (* TODO
-              hence es'_def:"es' = (vs_to_es ((take ln x32)@ves)) \<and> s' = s'' \<and> vs = vs' \<and> ln \<le> length x32"
+              hence es'_def:"es' = ((vs_to_es ((take ln x32)@ves)@[x31])) \<and> s' = s'' \<and> vs = vs' \<and> ln \<le> length x32"
                 using outer_outer_false False run_step_is Local 2(3) Suc
                 by (cases "ln \<le> length x32") auto
-              then obtain n lfilled es_c where local_eqs:"s=s'" "vs=vs'" "ln \<le> length x32" "Lfilled_exact n lfilled ((vs_to_es x32) @ [$Return] @ es_c) es"
-                using run_step_is run_step_return_imp_lfilled RSReturnCall
+              then obtain n lfilled es_c where local_eqs:"s=s'" "vs=vs'" "ln \<le> length x32" "Lfilled_exact n lfilled ((vs_to_es x32) @ [$ReturnCall j] @ es_c) es"
+                using run_step_is run_step_return_call_imp_lfilled RSReturnCall
                 by fastforce
-              then obtain lfilled' where lfilled_int:"Lfilled n lfilled' ((vs_to_es x32) @ [$Return]) es"
+              then obtain lfilled' where lfilled_int:"Lfilled n lfilled' ((vs_to_es x32) @ [$ReturnCall j]) es"
                 using lfilled_collapse2[OF Lfilled_exact_imp_Lfilled]
                 by fastforce
-              obtain lfilled'' where "Lfilled n lfilled'' ((drop (length x32 - ln) (vs_to_es x32)) @ [$Return]) es"
+              obtain lfilled'' where "Lfilled n lfilled'' ((drop (length x32 - ln) (vs_to_es x32)) @ [$ReturnCall j]) es"
                 using lfilled_collapse1[OF lfilled_int] is_const_list_vs_to_es_list[of "rev x32"] local_eqs(3)
                 by fastforce
               hence "\<lparr>[Local ln j vls es]\<rparr> \<leadsto> \<lparr>(drop (length x32 - ln) (vs_to_es x32))\<rparr>"
-                using reduce_simple.intros(44) local_eqs(3) is_const_list_vs_to_es_list
+                using reduce.intros(5) local_eqs(3) is_const_list_vs_to_es_list
                 unfolding drop_map
                 by fastforce
               hence 1:"\<lparr>s;vs;[Local ln j vls es]\<rparr> \<leadsto>_i \<lparr>s';vs';(drop (length x32 - ln) (vs_to_es x32))\<rparr>"
@@ -2646,7 +2965,6 @@ proof -
                 using es'_def
                 unfolding drop_map rev_take[symmetric]
                 by auto
-            *)
             next
               case (RSNormal x4)
               hence inner_reduce:"\<lparr>s;vls;es\<rparr> \<leadsto>_j \<lparr>s'';vls';x4\<rparr>"
@@ -2654,7 +2972,7 @@ proof -
                 by auto
               thus ?thesis
                 using Local 2(3) Local outer_outer_false False run_step_is Suc
-                      reduce.intros(24)[OF inner_reduce] RSNormal
+                      reduce.intros(27)[OF inner_reduce] RSNormal
                       progress_L0_left is_const_list_vs_to_es_list[of "rev ves"]
                 by (auto simp del: run_step.simps)
             qed
